\documentclass{article}
\usepackage{forest}
\usepackage[margin=1in]{geometry}
\newcommand{\comb}[1]{\textbf{\textsf{#1}}}
\usepackage[T1]{fontenc}
\begin{document}\scriptsize

\begin{forest}
for tree={parent anchor=south, child anchor=north, align=center}
[$\texttt{B t}$\\
{\comb{R}, \comb{>}}
[$\texttt{t -> t}$\\
\comb{Lex}
[\texttt{"not"}]]
[$\texttt{B t}$\\
{\comb{>}}
[$\texttt{B t -> B t}$\\
{\comb{>}}
[$\texttt{v -> B t -> B t}$\\
\comb{Lex}
[\texttt{"bexists"}]]
[$\texttt{v}$\\
\comb{Lex}
[\texttt{"x"}]]
]
[$\texttt{B t}$\\
{\comb{<}}
[$\texttt{B t}$\\
{\comb{>}}
[$\texttt{B (R t) -> B t}$\\
\comb{Lex}
[\texttt{"lower"}]]
[$\texttt{B (R t)}$\\
{\comb{R}, \comb{L}, \comb{>}}
[$\texttt{R (e -> t)}$\\
\comb{Lex}
[\texttt{"bathroom"}]]
[$\texttt{B e}$\\
\comb{Lex}
[\texttt{"x"}]]
]
]
[$\texttt{B t -> B t}$\\
{\comb{>}}
[$\texttt{B t -> B t -> B t}$\\
\comb{Lex}
[\texttt{"and"}]]
[$\texttt{B t}$\\
{\comb{D}, \comb{R}, \comb{>}}
[$\texttt{B (R t) -> B t}$\\
\comb{Lex}
[\texttt{"lower"}]]
[$\texttt{C (B (R t))}$\\
{\comb{L}, \comb{R}, \comb{L}, \comb{>}}
[$\texttt{C (R (e -> t))}$\\
{\comb{>}}
[$\texttt{R (e -> t) -> C (R (e -> t))}$\\
\comb{Lex}
[\texttt{"pfoc"}]]
[$\texttt{R (e -> t)}$\\
\comb{Lex}
[\texttt{"bathroom"}]]
]
[$\texttt{B e}$\\
\comb{Lex}
[\texttt{"x"}]]
]
]
]
]
]
]
\end{forest}


\bigskip
\begin{forest}
for tree={parent anchor=south, child anchor=north, align=center}
[$\texttt{B t}$\\
{\comb{R}, \comb{>}}
[$\texttt{t -> t}$\\
\comb{Lex}
[\texttt{"not"}]]
[$\texttt{B t}$\\
{\comb{>}}
[$\texttt{B t -> B t}$\\
{\comb{>}}
[$\texttt{v -> B t -> B t}$\\
\comb{Lex}
[\texttt{"bexists"}]]
[$\texttt{v}$\\
\comb{Lex}
[\texttt{"x"}]]
]
[$\texttt{B t}$\\
{\comb{D}, \comb{R}, \comb{<}}
[$\texttt{B t}$\\
{\comb{>}}
[$\texttt{B (R t) -> B t}$\\
\comb{Lex}
[\texttt{"lower"}]]
[$\texttt{B (R t)}$\\
{\comb{R}, \comb{L}, \comb{>}}
[$\texttt{R (e -> t)}$\\
\comb{Lex}
[\texttt{"bathroom"}]]
[$\texttt{B e}$\\
\comb{Lex}
[\texttt{"x"}]]
]
]
[$\texttt{C (B t -> B t)}$\\
{\comb{R}, \comb{>}}
[$\texttt{B t -> B t -> B t}$\\
\comb{Lex}
[\texttt{"and"}]]
[$\texttt{C (B t)}$\\
{\comb{R}, \comb{>}}
[$\texttt{B (R t) -> B t}$\\
\comb{Lex}
[\texttt{"lower"}]]
[$\texttt{C (B (R t))}$\\
{\comb{L}, \comb{R}, \comb{L}, \comb{>}}
[$\texttt{C (R (e -> t))}$\\
{\comb{>}}
[$\texttt{R (e -> t) -> C (R (e -> t))}$\\
\comb{Lex}
[\texttt{"pfoc"}]]
[$\texttt{R (e -> t)}$\\
\comb{Lex}
[\texttt{"bathroom"}]]
]
[$\texttt{B e}$\\
\comb{Lex}
[\texttt{"x"}]]
]
]
]
]
]
]
\end{forest}


\bigskip
\begin{forest}
for tree={parent anchor=south, child anchor=north, align=center}
[$\texttt{B t}$\\
{\comb{R}, \comb{>}}
[$\texttt{t -> t}$\\
\comb{Lex}
[\texttt{"not"}]]
[$\texttt{B t}$\\
{\comb{D}, \comb{R}, \comb{>}}
[$\texttt{B t -> B t}$\\
{\comb{>}}
[$\texttt{v -> B t -> B t}$\\
\comb{Lex}
[\texttt{"bexists"}]]
[$\texttt{v}$\\
\comb{Lex}
[\texttt{"x"}]]
]
[$\texttt{C (B t)}$\\
{\comb{R}, \comb{<}}
[$\texttt{B t}$\\
{\comb{>}}
[$\texttt{B (R t) -> B t}$\\
\comb{Lex}
[\texttt{"lower"}]]
[$\texttt{B (R t)}$\\
{\comb{R}, \comb{L}, \comb{>}}
[$\texttt{R (e -> t)}$\\
\comb{Lex}
[\texttt{"bathroom"}]]
[$\texttt{B e}$\\
\comb{Lex}
[\texttt{"x"}]]
]
]
[$\texttt{C (B t -> B t)}$\\
{\comb{R}, \comb{>}}
[$\texttt{B t -> B t -> B t}$\\
\comb{Lex}
[\texttt{"and"}]]
[$\texttt{C (B t)}$\\
{\comb{R}, \comb{>}}
[$\texttt{B (R t) -> B t}$\\
\comb{Lex}
[\texttt{"lower"}]]
[$\texttt{C (B (R t))}$\\
{\comb{L}, \comb{R}, \comb{L}, \comb{>}}
[$\texttt{C (R (e -> t))}$\\
{\comb{>}}
[$\texttt{R (e -> t) -> C (R (e -> t))}$\\
\comb{Lex}
[\texttt{"pfoc"}]]
[$\texttt{R (e -> t)}$\\
\comb{Lex}
[\texttt{"bathroom"}]]
]
[$\texttt{B e}$\\
\comb{Lex}
[\texttt{"x"}]]
]
]
]
]
]
]
\end{forest}


\bigskip
\begin{forest}
for tree={parent anchor=south, child anchor=north, align=center}
[$\texttt{B t}$\\
{\comb{D}, \comb{R}, \comb{R}, \comb{>}}
[$\texttt{t -> t}$\\
\comb{Lex}
[\texttt{"not"}]]
[$\texttt{C (B t)}$\\
{\comb{R}, \comb{>}}
[$\texttt{B t -> B t}$\\
{\comb{>}}
[$\texttt{v -> B t -> B t}$\\
\comb{Lex}
[\texttt{"bexists"}]]
[$\texttt{v}$\\
\comb{Lex}
[\texttt{"x"}]]
]
[$\texttt{C (B t)}$\\
{\comb{R}, \comb{<}}
[$\texttt{B t}$\\
{\comb{>}}
[$\texttt{B (R t) -> B t}$\\
\comb{Lex}
[\texttt{"lower"}]]
[$\texttt{B (R t)}$\\
{\comb{R}, \comb{L}, \comb{>}}
[$\texttt{R (e -> t)}$\\
\comb{Lex}
[\texttt{"bathroom"}]]
[$\texttt{B e}$\\
\comb{Lex}
[\texttt{"x"}]]
]
]
[$\texttt{C (B t -> B t)}$\\
{\comb{R}, \comb{>}}
[$\texttt{B t -> B t -> B t}$\\
\comb{Lex}
[\texttt{"and"}]]
[$\texttt{C (B t)}$\\
{\comb{R}, \comb{>}}
[$\texttt{B (R t) -> B t}$\\
\comb{Lex}
[\texttt{"lower"}]]
[$\texttt{C (B (R t))}$\\
{\comb{L}, \comb{R}, \comb{L}, \comb{>}}
[$\texttt{C (R (e -> t))}$\\
{\comb{>}}
[$\texttt{R (e -> t) -> C (R (e -> t))}$\\
\comb{Lex}
[\texttt{"pfoc"}]]
[$\texttt{R (e -> t)}$\\
\comb{Lex}
[\texttt{"bathroom"}]]
]
[$\texttt{B e}$\\
\comb{Lex}
[\texttt{"x"}]]
]
]
]
]
]
]
\end{forest}


\bigskip
\begin{forest}
for tree={parent anchor=south, child anchor=north, align=center}
[$\texttt{B t}$\\
{\comb{R}, \comb{>}}
[$\texttt{t -> t}$\\
\comb{Lex}
[\texttt{"not"}]]
[$\texttt{B t}$\\
{\comb{<}}
[$\texttt{B t}$\\
{\comb{>}}
[$\texttt{B t -> B t}$\\
{\comb{>}}
[$\texttt{v -> B t -> B t}$\\
\comb{Lex}
[\texttt{"bexists"}]]
[$\texttt{v}$\\
\comb{Lex}
[\texttt{"x"}]]
]
[$\texttt{B t}$\\
{\comb{>}}
[$\texttt{B (R t) -> B t}$\\
\comb{Lex}
[\texttt{"lower"}]]
[$\texttt{B (R t)}$\\
{\comb{R}, \comb{L}, \comb{>}}
[$\texttt{R (e -> t)}$\\
\comb{Lex}
[\texttt{"bathroom"}]]
[$\texttt{B e}$\\
\comb{Lex}
[\texttt{"x"}]]
]
]
]
[$\texttt{B t -> B t}$\\
{\comb{>}}
[$\texttt{B t -> B t -> B t}$\\
\comb{Lex}
[\texttt{"and"}]]
[$\texttt{B t}$\\
{\comb{D}, \comb{R}, \comb{>}}
[$\texttt{B (R t) -> B t}$\\
\comb{Lex}
[\texttt{"lower"}]]
[$\texttt{C (B (R t))}$\\
{\comb{L}, \comb{R}, \comb{L}, \comb{>}}
[$\texttt{C (R (e -> t))}$\\
{\comb{>}}
[$\texttt{R (e -> t) -> C (R (e -> t))}$\\
\comb{Lex}
[\texttt{"pfoc"}]]
[$\texttt{R (e -> t)}$\\
\comb{Lex}
[\texttt{"bathroom"}]]
]
[$\texttt{B e}$\\
\comb{Lex}
[\texttt{"x"}]]
]
]
]
]
]
\end{forest}


\bigskip
\begin{forest}
for tree={parent anchor=south, child anchor=north, align=center}
[$\texttt{B t}$\\
{\comb{R}, \comb{>}}
[$\texttt{t -> t}$\\
\comb{Lex}
[\texttt{"not"}]]
[$\texttt{B t}$\\
{\comb{D}, \comb{R}, \comb{<}}
[$\texttt{B t}$\\
{\comb{>}}
[$\texttt{B t -> B t}$\\
{\comb{>}}
[$\texttt{v -> B t -> B t}$\\
\comb{Lex}
[\texttt{"bexists"}]]
[$\texttt{v}$\\
\comb{Lex}
[\texttt{"x"}]]
]
[$\texttt{B t}$\\
{\comb{>}}
[$\texttt{B (R t) -> B t}$\\
\comb{Lex}
[\texttt{"lower"}]]
[$\texttt{B (R t)}$\\
{\comb{R}, \comb{L}, \comb{>}}
[$\texttt{R (e -> t)}$\\
\comb{Lex}
[\texttt{"bathroom"}]]
[$\texttt{B e}$\\
\comb{Lex}
[\texttt{"x"}]]
]
]
]
[$\texttt{C (B t -> B t)}$\\
{\comb{R}, \comb{>}}
[$\texttt{B t -> B t -> B t}$\\
\comb{Lex}
[\texttt{"and"}]]
[$\texttt{C (B t)}$\\
{\comb{R}, \comb{>}}
[$\texttt{B (R t) -> B t}$\\
\comb{Lex}
[\texttt{"lower"}]]
[$\texttt{C (B (R t))}$\\
{\comb{L}, \comb{R}, \comb{L}, \comb{>}}
[$\texttt{C (R (e -> t))}$\\
{\comb{>}}
[$\texttt{R (e -> t) -> C (R (e -> t))}$\\
\comb{Lex}
[\texttt{"pfoc"}]]
[$\texttt{R (e -> t)}$\\
\comb{Lex}
[\texttt{"bathroom"}]]
]
[$\texttt{B e}$\\
\comb{Lex}
[\texttt{"x"}]]
]
]
]
]
]
\end{forest}


\bigskip
\begin{forest}
for tree={parent anchor=south, child anchor=north, align=center}
[$\texttt{B t}$\\
{\comb{D}, \comb{R}, \comb{R}, \comb{>}}
[$\texttt{t -> t}$\\
\comb{Lex}
[\texttt{"not"}]]
[$\texttt{C (B t)}$\\
{\comb{R}, \comb{<}}
[$\texttt{B t}$\\
{\comb{>}}
[$\texttt{B t -> B t}$\\
{\comb{>}}
[$\texttt{v -> B t -> B t}$\\
\comb{Lex}
[\texttt{"bexists"}]]
[$\texttt{v}$\\
\comb{Lex}
[\texttt{"x"}]]
]
[$\texttt{B t}$\\
{\comb{>}}
[$\texttt{B (R t) -> B t}$\\
\comb{Lex}
[\texttt{"lower"}]]
[$\texttt{B (R t)}$\\
{\comb{R}, \comb{L}, \comb{>}}
[$\texttt{R (e -> t)}$\\
\comb{Lex}
[\texttt{"bathroom"}]]
[$\texttt{B e}$\\
\comb{Lex}
[\texttt{"x"}]]
]
]
]
[$\texttt{C (B t -> B t)}$\\
{\comb{R}, \comb{>}}
[$\texttt{B t -> B t -> B t}$\\
\comb{Lex}
[\texttt{"and"}]]
[$\texttt{C (B t)}$\\
{\comb{R}, \comb{>}}
[$\texttt{B (R t) -> B t}$\\
\comb{Lex}
[\texttt{"lower"}]]
[$\texttt{C (B (R t))}$\\
{\comb{L}, \comb{R}, \comb{L}, \comb{>}}
[$\texttt{C (R (e -> t))}$\\
{\comb{>}}
[$\texttt{R (e -> t) -> C (R (e -> t))}$\\
\comb{Lex}
[\texttt{"pfoc"}]]
[$\texttt{R (e -> t)}$\\
\comb{Lex}
[\texttt{"bathroom"}]]
]
[$\texttt{B e}$\\
\comb{Lex}
[\texttt{"x"}]]
]
]
]
]
]
\end{forest}


\bigskip
\begin{forest}
for tree={parent anchor=south, child anchor=north, align=center}
[$\texttt{B t}$\\
{\comb{<}}
[$\texttt{B t}$\\
{\comb{R}, \comb{>}}
[$\texttt{t -> t}$\\
\comb{Lex}
[\texttt{"not"}]]
[$\texttt{B t}$\\
{\comb{>}}
[$\texttt{B t -> B t}$\\
{\comb{>}}
[$\texttt{v -> B t -> B t}$\\
\comb{Lex}
[\texttt{"bexists"}]]
[$\texttt{v}$\\
\comb{Lex}
[\texttt{"x"}]]
]
[$\texttt{B t}$\\
{\comb{>}}
[$\texttt{B (R t) -> B t}$\\
\comb{Lex}
[\texttt{"lower"}]]
[$\texttt{B (R t)}$\\
{\comb{R}, \comb{L}, \comb{>}}
[$\texttt{R (e -> t)}$\\
\comb{Lex}
[\texttt{"bathroom"}]]
[$\texttt{B e}$\\
\comb{Lex}
[\texttt{"x"}]]
]
]
]
]
[$\texttt{B t -> B t}$\\
{\comb{>}}
[$\texttt{B t -> B t -> B t}$\\
\comb{Lex}
[\texttt{"and"}]]
[$\texttt{B t}$\\
{\comb{D}, \comb{R}, \comb{>}}
[$\texttt{B (R t) -> B t}$\\
\comb{Lex}
[\texttt{"lower"}]]
[$\texttt{C (B (R t))}$\\
{\comb{L}, \comb{R}, \comb{L}, \comb{>}}
[$\texttt{C (R (e -> t))}$\\
{\comb{>}}
[$\texttt{R (e -> t) -> C (R (e -> t))}$\\
\comb{Lex}
[\texttt{"pfoc"}]]
[$\texttt{R (e -> t)}$\\
\comb{Lex}
[\texttt{"bathroom"}]]
]
[$\texttt{B e}$\\
\comb{Lex}
[\texttt{"x"}]]
]
]
]
]
\end{forest}


\bigskip
\begin{forest}
for tree={parent anchor=south, child anchor=north, align=center}
[$\texttt{B t}$\\
{\comb{D}, \comb{R}, \comb{<}}
[$\texttt{B t}$\\
{\comb{R}, \comb{>}}
[$\texttt{t -> t}$\\
\comb{Lex}
[\texttt{"not"}]]
[$\texttt{B t}$\\
{\comb{>}}
[$\texttt{B t -> B t}$\\
{\comb{>}}
[$\texttt{v -> B t -> B t}$\\
\comb{Lex}
[\texttt{"bexists"}]]
[$\texttt{v}$\\
\comb{Lex}
[\texttt{"x"}]]
]
[$\texttt{B t}$\\
{\comb{>}}
[$\texttt{B (R t) -> B t}$\\
\comb{Lex}
[\texttt{"lower"}]]
[$\texttt{B (R t)}$\\
{\comb{R}, \comb{L}, \comb{>}}
[$\texttt{R (e -> t)}$\\
\comb{Lex}
[\texttt{"bathroom"}]]
[$\texttt{B e}$\\
\comb{Lex}
[\texttt{"x"}]]
]
]
]
]
[$\texttt{C (B t -> B t)}$\\
{\comb{R}, \comb{>}}
[$\texttt{B t -> B t -> B t}$\\
\comb{Lex}
[\texttt{"and"}]]
[$\texttt{C (B t)}$\\
{\comb{R}, \comb{>}}
[$\texttt{B (R t) -> B t}$\\
\comb{Lex}
[\texttt{"lower"}]]
[$\texttt{C (B (R t))}$\\
{\comb{L}, \comb{R}, \comb{L}, \comb{>}}
[$\texttt{C (R (e -> t))}$\\
{\comb{>}}
[$\texttt{R (e -> t) -> C (R (e -> t))}$\\
\comb{Lex}
[\texttt{"pfoc"}]]
[$\texttt{R (e -> t)}$\\
\comb{Lex}
[\texttt{"bathroom"}]]
]
[$\texttt{B e}$\\
\comb{Lex}
[\texttt{"x"}]]
]
]
]
]
\end{forest}



\end{document}