\documentclass{article}
\usepackage{forest}
\usepackage[margin=1in]{geometry}
\newcommand{\comb}[1]{\textbf{\textsf{#1}}}
\usepackage[T1]{fontenc}
\begin{document}\scriptsize

\begin{forest}
for tree={parent anchor=south, child anchor=north, align=center}
[$\texttt{R (g x w) (W t t)}$\\
{\comb{R}, \comb{R}, \comb{>}}
[$\texttt{t -> t}$\\
\comb{Lex}
[\texttt{"not"}]]
[$\texttt{R (g x w) (W t t)}$\\
{\comb{>}}
[$\texttt{R (g x w) (W t t) -> R (g x w) (W t t)}$\\
{\comb{>}}
[$\texttt{v -> R (g x w) (W t t) -> R (g x w) (W t t)}$\\
\comb{Lex}
[\texttt{"bexists"}]]
[$\texttt{v}$\\
\comb{Lex}
[\texttt{"x"}]]
]
[$\texttt{R (g x w) (W t t)}$\\
{\comb{D}, \comb{R}, \comb{>}}
[$\texttt{R (g x w) (W t (R w t)) -> R (g x w) (W t t)}$\\
\comb{Lex}
[\texttt{"lower"}]]
[$\texttt{C (R (g x w) (W t (R w t)))}$\\
{\comb{L}, \comb{R}, \comb{R}, \comb{L}, \comb{>}}
[$\texttt{C (R w (e -> t))}$\\
{\comb{>}}
[$\texttt{R w (e -> t) -> C (R w (e -> t))}$\\
\comb{Lex}
[\texttt{"pfoc"}]]
[$\texttt{R w (e -> t)}$\\
\comb{Lex}
[\texttt{"left"}]]
]
[$\texttt{R (g x w) (W t e)}$\\
\comb{Lex}
[\texttt{"x"}]]
]
]
]
]
\end{forest}


\bigskip
\begin{forest}
for tree={parent anchor=south, child anchor=north, align=center}
[$\texttt{R (g x w) (W t t)}$\\
{\comb{R}, \comb{R}, \comb{>}}
[$\texttt{t -> t}$\\
\comb{Lex}
[\texttt{"not"}]]
[$\texttt{R (g x w) (W t t)}$\\
{\comb{D}, \comb{R}, \comb{>}}
[$\texttt{R (g x w) (W t t) -> R (g x w) (W t t)}$\\
{\comb{>}}
[$\texttt{v -> R (g x w) (W t t) -> R (g x w) (W t t)}$\\
\comb{Lex}
[\texttt{"bexists"}]]
[$\texttt{v}$\\
\comb{Lex}
[\texttt{"x"}]]
]
[$\texttt{C (R (g x w) (W t t))}$\\
{\comb{R}, \comb{>}}
[$\texttt{R (g x w) (W t (R w t)) -> R (g x w) (W t t)}$\\
\comb{Lex}
[\texttt{"lower"}]]
[$\texttt{C (R (g x w) (W t (R w t)))}$\\
{\comb{L}, \comb{R}, \comb{R}, \comb{L}, \comb{>}}
[$\texttt{C (R w (e -> t))}$\\
{\comb{>}}
[$\texttt{R w (e -> t) -> C (R w (e -> t))}$\\
\comb{Lex}
[\texttt{"pfoc"}]]
[$\texttt{R w (e -> t)}$\\
\comb{Lex}
[\texttt{"left"}]]
]
[$\texttt{R (g x w) (W t e)}$\\
\comb{Lex}
[\texttt{"x"}]]
]
]
]
]
\end{forest}


\bigskip
\begin{forest}
for tree={parent anchor=south, child anchor=north, align=center}
[$\texttt{R (g x w) (W t t)}$\\
{\comb{D}, \comb{R}, \comb{R}, \comb{R}, \comb{>}}
[$\texttt{t -> t}$\\
\comb{Lex}
[\texttt{"not"}]]
[$\texttt{C (R (g x w) (W t t))}$\\
{\comb{R}, \comb{>}}
[$\texttt{R (g x w) (W t t) -> R (g x w) (W t t)}$\\
{\comb{>}}
[$\texttt{v -> R (g x w) (W t t) -> R (g x w) (W t t)}$\\
\comb{Lex}
[\texttt{"bexists"}]]
[$\texttt{v}$\\
\comb{Lex}
[\texttt{"x"}]]
]
[$\texttt{C (R (g x w) (W t t))}$\\
{\comb{R}, \comb{>}}
[$\texttt{R (g x w) (W t (R w t)) -> R (g x w) (W t t)}$\\
\comb{Lex}
[\texttt{"lower"}]]
[$\texttt{C (R (g x w) (W t (R w t)))}$\\
{\comb{L}, \comb{R}, \comb{R}, \comb{L}, \comb{>}}
[$\texttt{C (R w (e -> t))}$\\
{\comb{>}}
[$\texttt{R w (e -> t) -> C (R w (e -> t))}$\\
\comb{Lex}
[\texttt{"pfoc"}]]
[$\texttt{R w (e -> t)}$\\
\comb{Lex}
[\texttt{"left"}]]
]
[$\texttt{R (g x w) (W t e)}$\\
\comb{Lex}
[\texttt{"x"}]]
]
]
]
]
\end{forest}



\end{document}